low/RinternalsAux.v
@@ -11,11 +11,158 @@ Require Export Rinternals Shared.
  * instance [p_sym] for its [symSxp_struct] part—, that is [p->f] in C. **)
 
 
-(** * Instances **)
+(** * About the [nbits] Structure **)
 
-Instance SExpType_Comparable : Comparable SExpType.
-  prove_comparable_simple_inductive.
+Definition nth_bit {m : nat} (n : nat) : nbits m -> n < m -> bool.
+  introv a I. gen m. induction n as [|n]; introv a I; destruct m; try math.
+  - exact (fst a).
+  - applys IHn (snd a). math.
 Defined.
+Arguments nth_bit {m} n.
+
+(* A tactic to fill out the [n < m] part.
+ * The call to nth_bit should be on the form [nth_bit n a ltac:nbits_ok]. *)
+Ltac nbits_ok := repeat constructors.
+
+Lemma rewrite_nth_bit : forall n m (a : nbits m) (I I' : n < m),
+  nth_bit n a I = nth_bit n a I'.
+Proof.
+  induction n; introv; destruct m; try solve [ false; math ].
+  - reflexivity.
+  - simpl. erewrite IHn. reflexivity.
+Qed.
+
+Lemma rewrite_S_nth_bit : forall n m (a : nbits (S m)) (I : S n < S m) (I' : n < m),
+  nth_bit (S n) a I = nth_bit n (snd a) I'.
+Proof. introv. erewrite rewrite_nth_bit with (n := n). simpl. reflexivity. Qed.
+
+Definition write_nbit {m : nat} (n : nat) : nbits m -> n < m -> bool -> nbits m.
+  introv a I b. gen m. induction n as [|n]; introv a I; destruct m; try math.
+  - exact (b, snd a).
+  - refine (fst a, IHn _ (snd a) _). math.
+Defined.
+Arguments write_nbit {m} n.
+
+Lemma rewrite_write_nbit : forall n m (a : nbits m) (I I' : n < m) b,
+  write_nbit n a I b = write_nbit n a I' b.
+Proof.
+  induction n; introv; destruct m; try solve [ false; math ].
+  - reflexivity.
+  - simpl. erewrite IHn. reflexivity.
+Qed.
+
+Lemma rewrite_S_write_nbit : forall n m (a : nbits (S m)) (I : S n < S m) (I' : n < m) b,
+  write_nbit (S n) a I b = (fst a, write_nbit n (snd a) I' b).
+Proof. introv. erewrite rewrite_write_nbit with (n := n). simpl. reflexivity. Qed.
+
+Lemma write_nth_bit : forall n m (I : n < m) (a : nbits m) b,
+  nth_bit n (write_nbit n a I b) I = b.
+Proof.
+  induction n; introv; destruct m; try solve [ false; math ].
+  - reflexivity.
+  - asserts I': (n < m). math.
+    rewrite rewrite_S_nth_bit with (I' := I'). rewrite rewrite_S_write_nbit with (I' := I').
+    simpl. rewrite~ IHn.
+Qed.
+
+Fixpoint nbits_init (n : nat) : nbits n :=
+  match n with
+  | 0 => tt
+  | S n => (false, nbits_init n)
+  end.
+
+Lemma nbits_init_read : forall n m (I : n < m),
+  nth_bit n (nbits_init m) I = false.
+Proof.
+  induction n; introv; destruct m; try solve [ false; math ].
+  - reflexivity.
+  - asserts I': (n < m). math.
+    rewrite rewrite_S_nth_bit with (I' := I'). rewrite~ IHn.
+Qed.
+
+Definition nbits_to_list {n} (a : nbits n) : list bool.
+  induction n.
+  - exact nil.
+  - exact (fst a :: IHn (snd a)).
+Defined.
+
+Lemma nbits_to_list_length : forall n (a : nbits n),
+  length (nbits_to_list a) = n.
+Proof.
+  induction n; introv.
+  - reflexivity.
+  - simpl. rew_list. rewrite~ IHn.
+Qed.
+
+Lemma nbits_to_list_nth : forall n (a : nbits n) d m I,
+  nth_def d m (nbits_to_list a) = nth_bit m a I.
+Proof.
+  induction n; introv.
+  - false. math.
+  - destruct m as [|m].
+    + reflexivity.
+    + simpl. erewrite~ IHn.
+Qed.
+
+Fixpoint list_to_nbits (l : list bool) : nbits (length l) :=
+  match l return nbits (length l) with
+  | nil => tt
+  | b :: l => (b, list_to_nbits l)
+  end.
+
+Lemma list_to_nbits_to_list : forall l,
+  nbits_to_list (list_to_nbits l) = l.
+Proof.
+  introv. induction l.
+  - reflexivity.
+  - simpl. fequals~.
+Qed.
+
+Definition nbits_to_nat {n} (a : nbits n) : nat.
+  induction n.
+  - exact 0.
+  - exact ((if fst a then 1 else 0) + 2 * IHn (snd a)).
+Defined.
+(** Important note: the first bit in this representation has the lower weight. **)
+
+Lemma rewrite_nbits_to_nat : forall n (a : nbits (S n)),
+  nbits_to_nat a = ((if fst a then 1 else 0) + 2 * nbits_to_nat (snd a)).
+Proof. reflexivity. Qed.
+
+Definition nat_to_nbits {n} m : m < 2 ^ n -> nbits n.
+  introv I'. asserts I: (m < 2 ^ n)%nat. math.
+  clear I'. gen m. induction n; introv I.
+  - exact tt.
+  - refine (decide (m mod 2 = 1), IHn (m / 2) _).
+    apply~ Nat.div_lt_upper_bound.
+Defined.
+Arguments nat_to_nbits {n} m.
+
+Lemma rewrite_nat_to_nbits : forall n m I I',
+  nat_to_nbits m I = (nat_to_nbits m I' : nbits n).
+Proof.
+  induction n; introv.
+  - reflexivity.
+  - unfolds. fequals.
+Qed.
+
+Lemma rewrite_nat_to_nbits_cons : forall n m I I',
+  nat_to_nbits m I = ((decide (m mod 2 = 1), nat_to_nbits (m / 2) I') : nbits (S n)).
+Proof. introv. unfold nat_to_nbits. simpl. repeat fequals. Qed.
+
+Lemma nat_to_nbits_to_nat : forall n m I,
+  nbits_to_nat (nat_to_nbits m I : nbits n) = m.
+Proof.
+  introv. gen m. induction n; introv.
+  - simpls. math.
+  - asserts I1: (m / 2 < 2 ^ n)%nat. apply~ Nat.div_lt_upper_bound. simpl in I. math.
+    asserts I2: (m / 2 < 2 ^ n). math.
+    rewrite rewrite_nat_to_nbits_cons with (I' := I2). rewrite rewrite_nbits_to_nat.
+    unfold snd, fst. rewrite IHn.
+    rewrite Nat.div_mod with (y := 2); [|math]. rewrite Nat.add_comm. fequals.
+    clear. forwards I: Nat.mod_upper_bound m 2. math.
+    destruct (m mod 2); cases_if as M; fold_bool; rew_refl in M; try math.
+Qed.
 
 
 (** * Accessors and Smart Constructors **)
@@ -112,21 +259,6 @@ Definition get_promSxp e_ :=
   | _ => None
   end.
 
-Definition nth_bit {m : nat} (n : nat) : nbits m -> n < m -> bool.
-Defined.
-
-Definition write_nbit {m : nat} (n : nat) : nbits m -> n < m -> bool -> nbits m.
-Defined.
-
-Fixpoint nbits_init (n : nat) : nbits n :=
-  match n with
-  | 0 => tt
-  | S n => (false, nbits_init n)
-  end.
-
-(* A tactic to fill out the [n < m] part.
- * The call to nth_bit should be on the form [nth_bit n a ltac:nbits_ok]. *)
-Ltac nbits_ok := repeat constructors.
 
 Definition set_named_sxpinfo n i_info :=
   make_SxpInfo (type i_info) (obj i_info) n (gp i_info)
@@ -150,27 +282,27 @@ Definition map_sxpinfo_Vector_SExpRec T f (e_ : Vector_SExpRec T) :=
        (attrib h)
        (**gengc_prev_node h**)
        (**gengc_next_node h**))
-    (Vector_SExpRec_data e_).
+    (Vector_SExpRec_vecsxp e_).
 
 Definition map_sxpinfo f e_ :=
   match e_ with
   | SExpRec_NonVector e_ =>
-    SExpRec_NonVector (map_sxpinfo_NonVector_SExpRec e_)
+    SExpRec_NonVector (map_sxpinfo_NonVector_SExpRec f e_)
   | SExpRec_VectorChar e_ =>
-    SExpRec_VectorChar (map_sxpinfo_Vector_SExpRec e_)
+    SExpRec_VectorChar (map_sxpinfo_Vector_SExpRec f e_)
   | SExpRec_VectorLogical e_ =>
-    SExpRec_VectorLogical (map_sxpinfo_Vector_SExpRec e_)
+    SExpRec_VectorLogical (map_sxpinfo_Vector_SExpRec f e_)
   | SExpRec_VectorInteger e_ =>
-    SExpRec_VectorInteger (map_sxpinfo_Vector_SExpRec e_)
+    SExpRec_VectorInteger (map_sxpinfo_Vector_SExpRec f e_)
   | SExpRec_VectorComplex e_ =>
-    SExpRec_VectorComplex (map_sxpinfo_Vector_SExpRec e_)
+    SExpRec_VectorComplex (map_sxpinfo_Vector_SExpRec f e_)
   | SExpRec_VectorReal e_ =>
-    SExpRec_VectorReal (map_sxpinfo_Vector_SExpRec e_)
+    SExpRec_VectorReal (map_sxpinfo_Vector_SExpRec f e_)
   | SExpRec_VectorPointers e_ =>
-    SExpRec_VectorPointers (map_sxpinfo_Vector_SExpRec e_)
+    SExpRec_VectorPointers (map_sxpinfo_Vector_SExpRec f e_)
   end.
 
-Definition set_named n e_ :=
+Definition set_named n :=
   map_sxpinfo (set_named_sxpinfo n).
 
 Definition set_named_plural :=
@@ -180,10 +312,8 @@ Definition set_type_sxpinfo t i_info :=
   make_SxpInfo t (obj i_info) (named i_info) (gp i_info)
     (**mark i_info**) (**debug i_info**) (**trace i_info**) (**spare i_info**) (**gcgen i_info**).
 
-Definition set_type t e_ :=
+Definition set_type t :=
   map_sxpinfo (set_type_sxpinfo t).
-
-Definition set_gp := ?.
 
 Definition set_car_list car l_list :=
   make_ListSxp_struct car (list_cdrval l_list) (list_tagval l_list).
@@ -198,84 +328,117 @@ Definition build_SxpInfo type : SxpInfo :=
  * allocation is not targetted by this formalisation. We thus offer the
  * following smart constructor for the type [SExpRecHeader]. **)
 Definition build_SExpRecHeader type attrib : SExpRecHeader :=
-  make_SExpRecHeader (build_SxpInfo type) attrib None None.
+  make_SExpRecHeader (build_SxpInfo type) attrib (**None**) (**None**).
 
+(* This object seems to be just NULL.
 (** The Nil object TODO **)
 Definition Nil_SExpRec :=
-  make_SExpRec
+  make_NonVector_SExpRec
     (make_SExpRecHeader NilSxp None)
     ?.
+*)
 
 (** Smart constructors for each R data type. **)
 
 Definition make_SExpRec_sym attrib pname value internal :=
   SExpRec_NonVector
-    (make_SExpRec (build_SExpRecHeader SymSxp attrib)
+    (make_NonVector_SExpRec (build_SExpRecHeader SymSxp attrib)
       (make_SymSxp_struct pname value internal)).
 
 Definition make_SExpRec_list attrib car cdr tag :=
   SExpRec_NonVector
-    (make_SExpRec (build_SExpRecHeader ListSxp attrib)
+    (make_NonVector_SExpRec (build_SExpRecHeader ListSxp attrib)
       (make_ListSxp_struct car cdr tag)).
 
 Definition make_SExpRec_clo attrib formals body env :=
   SExpRec_NonVector
-    (make_SExpRec (build_SExpRecHeader CloSxp attrib)
+    (make_NonVector_SExpRec (build_SExpRecHeader CloSxp attrib)
       (make_CloSxp_struct formals body env)).
 
 Definition make_SExpRec_env attrib frame enclos (** hashtab **) :=
   SExpRec_NonVector
-    (make_SExpRec (build_SExpRecHeader EnvSxp attrib)
+    (make_NonVector_SExpRec (build_SExpRecHeader EnvSxp attrib)
       (make_EnvSxp_struct frame enclos)).
 
 Definition make_SExpRec_prom attrib value expr env :=
   SExpRec_NonVector
-    (make_SExpRec (build_SExpRecHeader CloSxp attrib)
+    (make_NonVector_SExpRec (build_SExpRecHeader CloSxp attrib)
       (make_CloSxp_struct value expr env)).
 
 Definition make_SExpRec_lang attrib function argumentList :=
   SExpRec_NonVector
-    (make_SExpRec (build_SExpRecHeader LangSxp attrib)
-      (make_ListSxp_struct function argumentList R_NilValue)).
+    (make_NonVector_SExpRec (build_SExpRecHeader LangSxp attrib)
+      (make_ListSxp_struct function argumentList None)).
 
 Definition make_SExpRec_prim attrib prim :=
   SExpRec_NonVector
-    (make_SExpRec (build_SExpRecHeader
+    (make_NonVector_SExpRec (build_SExpRecHeader
         match prim with
-        | primitive_construction_primitive => BuiltinSxp
-        | primitive_construction_internal => SpecialSxp
+        | primitive_construction_primitive _ => BuiltinSxp
+        | primitive_construction_internal _ => SpecialSxp
         end attrib)
-      (make_PrimSxp_struct prim).
+      (make_PrimSxp_struct prim)).
 
 Definition make_SExpRec_char attrib array :=
-  SExpRec_VectorChar (build_SExpRecHeader CharSxp attrib)
-    (make_Vector_SExpRec (length array) array).
+  SExpRec_VectorChar
+    (make_Vector_SExpRec
+      (build_SExpRecHeader CharSxp attrib)
+      (make_VecSxp_struct (length array) array)).
 
-Definition make_SExpRec_lgl attrib arr :=
-  SExpRec_VectorLogical (build_SExpRecHeader LglSxp attrib)
-    (make_Vector_SExpRec (length array) array).
+Definition make_SExpRec_lgl attrib array :=
+  SExpRec_VectorLogical
+    (make_Vector_SExpRec
+      (build_SExpRecHeader LglSxp attrib)
+      (make_VecSxp_struct (length array) array)).
 
-Definition make_SExpRec_int attrib arr :=
-  SExpRec_VectorInteger (build_SExpRecHeader IntSxp attrib)
-    (make_Vector_SExpRec (length array) array).
+Definition make_SExpRec_int attrib array :=
+  SExpRec_VectorInteger
+    (make_Vector_SExpRec
+      (build_SExpRecHeader IntSxp attrib)
+      (make_VecSxp_struct (length array) array)).
 
-Definition make_SExpRec_real attrib arr :=
-  SExpRec_VectorReal (build_SExpRecHeader RealSxp attrib)
-    (make_Vector_SExpRec (length array) array).
+Definition make_SExpRec_real attrib array :=
+  SExpRec_VectorReal
+    (make_Vector_SExpRec
+      (build_SExpRecHeader RealSxp attrib)
+      (make_VecSxp_struct (length array) array)).
 
-Definition make_SExpRec_cpl attrib arr :=
-  SExpRec_VectorComplex (build_SExpRecHeader CplSxp attrib)
-    (make_Vector_SExpRec (length array) array).
+Definition make_SExpRec_cpl attrib array :=
+  SExpRec_VectorComplex
+    (make_Vector_SExpRec
+      (build_SExpRecHeader CplxSxp attrib)
+      (make_VecSxp_struct (length array) array)).
 
-Definition make_SExpRec_str attrib arr :=
-  SExpRec_VectorPointers (build_SExpRecHeader StrSxp attrib)
-    (make_Vector_SExpRec (length array) array).
+Definition make_SExpRec_str attrib array :=
+  SExpRec_VectorPointers
+    (make_Vector_SExpRec
+      (build_SExpRecHeader StrSxp attrib)
+      (make_VecSxp_struct (length array) array)).
 
-Definition make_SExpRec_vec attrib arr :=
-  SExpRec_VectorPointers (build_SExpRecHeader VecSxp attrib)
-    (make_Vector_SExpRec (length array) array).
+Definition make_SExpRec_vec attrib array :=
+  SExpRec_VectorPointers
+    (make_Vector_SExpRec
+      (build_SExpRecHeader VecSxp attrib)
+      (make_VecSxp_struct (length array) array)).
 
-Definition make_SExpRec_expr attrib arr :=
-  SExpRec_VectorPointers (build_SExpRecHeader ExprSxp attrib)
-    (make_Vector_SExpRec (length array) array).
+Definition make_SExpRec_expr attrib array :=
+  SExpRec_VectorPointers
+    (make_Vector_SExpRec
+      (build_SExpRecHeader ExprSxp attrib)
+      (make_VecSxp_struct (length array) array)).
+
+
+(** * Instances **)
+
+Instance SExpType_Comparable : Comparable SExpType.
+  prove_comparable_simple_inductive.
+Defined.
+
+Instance SExpRec_Inhab : Inhab SExpRec.
+  apply prove_Inhab.
+  refine (make_NonVector_SExpRec
+            (make_SExpRecHeader (make_SxpInfo NilSxp false named_plural (nbits_init _)) None)
+            (make_ListSxp_struct None None None)). (* May not be the best choice. *)
+Defined.
+
 
