high/Rreasoning.v
@@ -1,4 +1,0 @@
-(** Rreasoning.
- * Definitions and tools to reason about R programs. **)
-
-
